theories/Commons/Values.v
@@ -1,6 +1,9 @@
 From RSL Require Import Prelude.
 
+From stdpp Require Import gmap.
+
 Definition loc : Type := positive.
+Definition loc_map : Type := gset (loc * loc).
 
 Variant val : Type :=
 | VInt (v: Z)
@@ -8,10 +11,28 @@ Variant val : Type :=
 | VPtr (l : loc)
 | VUndef.
 
-Definition val_eq (loc_eq : loc -> loc -> Prop) (v1 v2 : val) :=
-  match v1, v2 with
-  | VInt i1, VInt i2 => i1 = i2
-  | VBool b1, VBool b2 => b1 = b2
-  | VPtr p1, VPtr p2 => loc_eq p1 p2
-  | _, _ => False
-  end.
+Definition related (I: loc_map) l1 l2 :=
+  (l2, l1) ∈ I.
+
+Variant same_val I : val -> val -> Prop :=
+  | IntEq i1 i2:
+    i1 = i2 ->
+    same_val I (VInt i1) (VInt i2)
+
+  | BoolEq b1 b2:
+    b1 = b2 ->
+    same_val I (VBool b1) (VBool b2)
+
+  | PtrEq p1 p2:
+    related I p1 p2 ->
+    same_val I (VPtr p1) (VPtr p2).
+
+Lemma same_val_mono I I' vt vs :
+  I ⊆ I' ->
+  same_val I vt vs ->
+  same_val I' vt vs.
+Proof using Type.
+  intros Hincl Hsame.
+  inv Hsame; econstructor; auto.
+  by apply Hincl.
+Qed.
