theories/Playground/Optim.v
@@ -5,69 +5,68 @@ From RSL.RTL Require Import SimRules.
 
 Import RTLNotations.
 
-Section T.
-  Let Λt : lang := rtl_lang.
-  Let Λs : lang := rtl_lang.
+Definition no_opt_fun (fs: rtl_function) : rtl_function :=
+  {|
+    fn_name := fn_name fs;
+    fn_regs := fn_regs fs;
+    fn_entrypoint := fn_entrypoint fs;
+    fn_code := fn_code fs;
+    fn_regs_no_dup := fn_regs_no_dup fs
+  |}.
 
-  Definition no_opt_fun (fs: rtl_function) : rtl_function :=
-    {|
-      fn_name := fn_name fs;
-      fn_regs := fn_regs fs;
-      fn_entrypoint := fn_entrypoint fs;
-      fn_code := fn_code fs;
-      fn_regs_no_dup := fn_regs_no_dup fs
-    |}.
+Lemma no_opt_no_dup {Ps}:
+  is_no_dup (fn_name <$> prog_fun_list Ps) = true ->
+  is_no_dup (fn_name <$> fmap no_opt_fun (prog_fun_list Ps)) = true.
+Proof using Type.
+  rewrite !is_no_dup_sound.
+  induction (prog_fun_list Ps) as [ | f l IH ].
+  - done.
+  - simpl. intros H. inv H as [| ? ? HnIn HnDup].
+    constructor; auto.
+    intros (? & Heq & (f' & -> & H)%list_elem_of_fmap)%list_elem_of_fmap.
+    apply HnIn. rewrite Heq.
+    apply list_elem_of_fmap.
+    by exists f'.
+Qed.
 
-  Lemma no_opt_no_dup {Ps} :
-    is_no_dup (fn_name <$> prog_fun_list Ps) = true ->
-    is_no_dup (fn_name <$> fmap no_opt_fun (prog_fun_list Ps)) = true.
-  Proof using Type.
-    rewrite !is_no_dup_sound.
-    induction (prog_fun_list Ps) as [ | f l IH ].
-    - done.
-    - simpl. intros H. inv H as [| ? ? HnIn HnDup].
-      constructor; auto.
-      intros (? & Heq & (f' & -> & H)%list_elem_of_fmap)%list_elem_of_fmap.
-      apply HnIn. rewrite Heq.
-      apply list_elem_of_fmap.
-      by exists f'.
-  Qed.
+Lemma no_opt_find_fun_list {Ps} fn f:
+  find_fun_in_list (prog_fun_list Ps) fn = Some f ->
+  find_fun_in_list (no_opt_fun <$> prog_fun_list Ps) fn = Some (no_opt_fun f).
+Proof using Type.
+  unfold find_fun_in_list.
+  intros ([? f'] & H & Heq)%fmap_Some. simpl in Heq. subst f'.
+  apply list_find_Some in H as (Hres & Hp & Hfirst).
+  rewrite fmap_Some. eexists (_, _). split; last reflexivity.
+  apply list_find_Some. split_and!.
+  - apply list_lookup_fmap_Some. by eexists.
+  - done.
+  - intros j ? (f' & -> & Hin)%list_lookup_fmap_Some Hj. simpl.
+    by eapply Hfirst.
+Qed.
 
-  Lemma no_opt_with_main {Ps} :
-    is_Some (find_fun_in_list (prog_fun_list Ps) (prog_main Ps)) ->
-    is_Some (find_fun_in_list (no_opt_fun <$> prog_fun_list Ps) (prog_main Ps)).
-  Proof using Type.
-    unfold find_fun_in_list.
-    intros [fmain ([n f] & H & ->)%fmap_Some].
-    apply list_find_Some in H as (Hres & Hp & Hfirst).
-    rewrite fmap_is_Some.
-    eexists (_, _).
-    apply list_find_Some. split_and!.
-    - apply list_lookup_fmap_Some. by exists f.
-    - done.
-    - intros j ? (f' & -> & Hin)%list_lookup_fmap_Some Hj. simpl.
-      by eapply Hfirst.
-  Qed.
+Lemma no_opt_main_some {Ps}:
+  is_Some (find_fun_in_list (prog_fun_list Ps) (prog_main Ps)) ->
+  is_Some (find_fun_in_list (no_opt_fun <$> prog_fun_list Ps) (prog_main Ps)).
+Proof using Type.
+  intros [f H]. eexists. by apply no_opt_find_fun_list.
+Qed.
 
-  Definition no_opt (Ps: prog Λs) : prog Λt :=
-    {|
-      prog_fun_list := fmap no_opt_fun (prog_fun_list Ps);
-      prog_main := prog_main Ps;
-      prog_fun_list_no_dup := no_opt_no_dup (prog_fun_list_no_dup Ps);
-      prog_main_exists := no_opt_with_main (prog_main_exists Ps)
-    |}.
+Definition no_opt (Ps: rtl_program) : rtl_program :=
+  {|
+    prog_fun_list := fmap no_opt_fun (prog_fun_list Ps);
+    prog_main := prog_main Ps;
+    prog_fun_list_no_dup := no_opt_no_dup (prog_fun_list_no_dup Ps);
+    prog_main_exists := no_opt_main_some (prog_main_exists Ps)
+  |}.
 
-  Context (Ps : prog Λs).
-  Let Pt : prog Λt := no_opt Ps.
+Lemma no_opt_find_fun {Ps} fn f:
+  find_fun Ps fn = Some f ->
+  find_fun (no_opt Ps) fn = Some (no_opt_fun f).
+Proof using Type. by apply no_opt_find_fun_list. Qed.
 
-  Definition no_opt_inv (st: pstate Λt) (j i: nat) (ss: pstate Λs) ϕ : rProp :=
-    ∃ I f pc ρt ρs,
-      ⌜st = ([], State (no_opt_fun f) pc ρt)⌟ ∗
-      ⌜ss = ([], State f pc ρs)⌟ ∗
-      ⌜∀ r, ρt@r <{ I }> ρs@r⌟ ∗
-      mem_inj I ∅ ∗
-      (∀ vt vs : value rtl_lang,
-         (∃ I', ⌜ I ⊆ I' ⌟ ∗ ⌜ same_val I' vt vs ⌟ ∗ mem_inj I' ∅) -∗ ϕ vt vs).
+Section no_opt.
+  Context (Ps : rtl_program).
+  Let Pt := no_opt Ps.
 
   Definition same_args I valt vals : rProp :=
     ⌜Forall2 (same_val I) valt vals⌟ ∗ mem_inj I ∅.
@@ -75,68 +74,122 @@ Section T.
   Definition samer I vt vs : rProp :=
     ∃ I', ⌜I ⊆ I'⌟ ∗ ⌜same_val I' vt vs⌟ ∗ mem_inj I' ∅.
 
-  Lemma toto_no_opt C f I :
+  Lemma samer_mono I I' vt vs:
+    I ⊆ I' ->
+    samer I' vt vs -∗
+    samer I vt vs.
+  Proof using Type.
+    iIntros (Hincl) "(%I'' & %Hinl' & Hsame & Hinj)".
+    iExists I''. iFrame. iPureIntro.
+    by transitivity I'.
+  Qed.
+
+  Definition no_opt_sim_inv : SInv rtl_lang rtl_lang WfNat WfNat :=
+    fun st j i ss ϕ =>
+      (∃ I f pc ρt ρs,
+          ⌜st = ([], State (no_opt_fun f) pc ρt)⌟ ∗
+          ⌜ss = ([], State f pc ρs)⌟ ∗
+          ⌜∀ r, ρt@r <{ I }> ρs@r⌟ ∗
+          mem_inj I ∅ ∗
+          (∀ vt vs, samer I vt vs -∗ ϕ vt vs)
+      )%I.
+
+  Lemma no_opt_lemma C f I :
     ⊢ [Pt, Ps, C] {{ same_args I }} (no_opt_fun f) <{0, 0}= f {{ samer I }}.
   Proof using Type.
-    iIntros "!>" (valt vals ϕ) "[%Harg Hinj] Hpost".
+    iIntros "!>" (valt vals Ψ) "[%Harg Hinj] Hpost".
     iApply (source_callstate_exploit).
     iIntros (ρs pc Hlen -> ->).
-    iApply (target_callstate); auto. { by eapply Forall2_length_r. }
+    iApply (target_callstate); auto; first by eapply Forall2_length_r.
     simpl.
-    iApply (coind no_opt_inv).
+    iApply (coind no_opt_sim_inv).
     {
-      clear. iIntros "!>" (C st j i ss ϕ) "#CIH".
+      clear.
+      iIntros "!>" (C st j i ss ϕ) "#CIH".
       iIntros "(%I & %f & %pc & %ρt & %ρs & -> & -> & %Hsame & Hinj & Hpost)".
       destruct ((fn_code f) !! pc)
         as [
           [ pc'
-          | op args pc'
+          | op args dst pc'
           | src dst pc'
           | dst src pc'
-          | fn args dst pc'
-          | b tpc fpc
+          | fname args dst pc'
+          | r tpc fpc
           | r
           ]
         |] eqn:Hi.
-      - iApply (source_nop). { done. }
-        iApply (target_nop). { done. }
+      - iApply (source_nop); try done.
+        iApply (target_nop); try done.
         iApply "CIH"; try (iPureIntro; simpl; lia).
         iExists I, f, _, ρt, ρs. iFrame. iPureIntro. by split_and!.
-      - destruct (regbank_never_empty_list ρs args) as [vs].
-        destruct (regbank_never_empty_list ρt args) as [vt].
+
+      - destruct (regbank_never_empty_list ρs args) as [vs Hvs].
+        destruct (regbank_never_empty_list ρt args) as [vt Hvt].
         iApply (source_op_exploit); try done.
-        iIntros (v Hv). iApply (target_op).
-        { done. }
-        { done. }
-        { admit. }
-        iApply "CIH"; try (iPureIntro; simpl; lia).
-        iExists I, f, _, _, _. iFrame. iPureIntro. split_and!. 1-2: done.
-        { admit. }
+        iIntros (v Hv). iApply (target_op); try done.
+        + instantiate (1 := v). admit.
+        + iApply "CIH"; try (iPureIntro; simpl; lia).
+          iExists I, f, _, _, _. iFrame. iPureIntro. split_and!; try done.
+          intros r.
+          admit.
+
       - destruct (Hsame src) as (vt & vs & Ht & Hs & Hv).
         iApply (both_load with "[Hpost] Hinj"); try done.
         iIntros (vt' vs' Hv') "Hinj".
         iApply "CIH"; try (iPureIntro; simpl; lia).
-        iExists I, f, _, _, _. iFrame. iPureIntro. split_and!. 1-2: done.
-        { admit. }
+        iExists I, f, _, _, _. iFrame. iPureIntro. split_and!; try done.
+        admit.
+
       - destruct (Hsame src) as (addrt & addrs & Haddrt & Haddrs & Haddr).
         destruct (Hsame dst) as (dstt & dsts & Hdstt & Hdsts & Hdst).
         iApply (both_store with "[Hpost] Hinj"); try done.
         iIntros "Hinj".
         iApply "CIH"; try (iPureIntro; simpl; lia).
         iExists I, f, _, _, _. iFrame. iPureIntro. by split_and!.
-      - destruct (find_fun Ps fn) eqn:Hfn.
-        + destruct (regbank_never_empty_list ρs args) as [vs].
-          destruct (regbank_never_empty_list ρt args) as [vt].
-          iApply (both_call_framed); try done.
-          { admit. }
-          { admit. }
-          { admit. }
-          { admit. }
-        + iApply (source_call_fails); eauto. iCombine "Hinj Hpost" as "H". iApply "H".
-      - admit.
-      - admit.
-      - iApply (source_fails). { done. }
-        iCombine "Hinj Hpost" as "H". iApply "H".
+
+      - destruct (find_fun Ps fname) as [fn |] eqn:Hfn; last by iApply (source_call_fail).
+        destruct (regbank_never_empty_list ρs args) as [vs].
+        destruct (regbank_never_empty_list ρt args) as [vt].
+        iApply (both_call_framed (same_args I) (samer I) with "[] [Hinj] Hpost"); eauto.
+        + by apply no_opt_find_fun.
+        + clear.
+          iIntros "!>" (valt vals Ψ) "[%Harg Hinj] Hpost".
+          iApply (source_callstate_exploit).
+          iIntros (ρs pc Hlen -> ->).
+          iApply (target_callstate); auto; first by eapply Forall2_length_r.
+          iApply "CIH"; simpl; try (iPureIntro; lia).
+          iExists I, fn, _, _, _.  iFrame. iPureIntro.
+          split_and!.
+          * done.
+          * done.
+          * intros r.
+            admit.
+        + iFrame. iPureIntro.
+          admit.
+        + iIntros "!>" (j' i' ? ? ? ?) "(%I' & %Hincl & %Hsame' & Hinj) Hpost".
+          iApply "CIH"; auto.
+          iExists I', f, _, _, _. iFrame.
+          iSplitR. { by iPureIntro. }
+          iSplitR. { by iPureIntro. }
+          iSplitR.
+          * iPureIntro. intros r.
+            admit.
+          * iIntros (? ?) "Hsame". iApply "Hpost". by iApply (samer_mono with "Hsame").
+
+      - destruct (Hsame r) as (bt & bs & Hbt & Hbs & Hb).
+        iApply (source_if_exploit); try done.
+        iIntros (b pc' -> ->). inv Hb.
+        iApply (target_if); try done.
+        iApply "CIH"; simpl; try (iPureIntro; lia).
+        iExists I, _, _, _, _.  iFrame. iPureIntro. by split_and!.
+
+      - destruct (Hsame r) as (vt & vs & Hvt & Hvs & Hr).
+        iApply (source_ret); try done.
+        iApply (target_ret); try done.
+        iApply (both_ret). iApply "Hpost".
+        iExists I. iFrame. by iPureIntro.
+
+      - by iApply (source_fail).
     }
     iExists I, f, _, _, _. iFrame.
     iPureIntro. split_and!.
@@ -145,4 +198,4 @@ Section T.
     - intros r.
       admit.
   Admitted.
-End T.
+End no_opt.
