theories/RTL/Rules/FailSourceRules.v
@@ -1,0 +1,61 @@
+From RSL Require Import Prelude.
+
+From RSL.RTL Require Import RTL Semantics.
+From RSL.RTL.Rules Require Import SourceRules.
+From RSL.Logic Require Import Logic.
+
+Import RTLNotations.
+
+Section FailingSourceRulesDef.
+  Context {Λt : lang}.
+  Let Λs : lang := rtl_lang.
+  Context {Pt : prog Λt} {Ps : prog Λs}.
+  Context {C : Chain (fsim_lfp WfNat WfNat Pt Ps)}.
+
+  Context (st : pstate Λt) (j i : WfNat) (cs : list stackframe)
+    (fs : rtl_function) (pcs : node) (ρs : regbank)
+    (Q : value Λt -> value Λs -> rProp).
+
+  Lemma source_fail :
+    (fn_code fs) !! pcs = None ->
+    True -∗
+    [Pt, Ps, C] st <{j, i}= (cs, State fs pcs ρs) {{ Q }}.
+  Proof using Type.
+    intros Hpc. unseal.
+    intros ? ? [-> ->] mt ms _ _ _. smap.
+    source_does_UB.
+  Qed.
+
+  Lemma source_op_fail pc dst op regs args:
+    fs@pcs is <<{ dst := @op regs -> pc }>> ->
+    ρs @ regs ⇒ args ->
+    eval_op op args = None ->
+    True -∗
+    [Pt, Ps, C] st <{j, i}= (cs, State fs pcs ρs) {{ Q }}.
+  Proof using Type.
+    intros Hpc Hargs Hv. unseal.
+    intros ? ? [-> ->] mt ms _ _ _. smap.
+    source_does_UB.
+  Qed.
+
+  Lemma source_call_fail dst sig args pc' :
+    fs@pcs is <<{ dst := @call sig args -> pc' }>> ->
+    find_fun Ps sig = None ->
+    True -∗
+    [Pt, Ps, C] st <{j, i}= (cs, State fs pcs ρs) {{ Q }}.
+  Proof using Type.
+    intros Hpc Hfun. unseal.
+    intros ? ? [-> ->] mtP msP _ _ Hsim. smap.
+    source_does_UB.
+  Qed.
+
+  Lemma source_callstate_fail args:
+    length args ≠ length (fn_regs fs) ->
+    True -∗
+    [Pt, Ps, C] st <{j, i}= (cs, CallState fs args) {{ Q }}.
+  Proof using Type.
+    intros Hlen. unseal.
+    intros ? ? [-> ->] mt ms _ _ Hsim. smap.
+    source_does_UB.
+  Qed.
+End FailingSourceRulesDef.
