theories/RTL/Rules/Hoare.v
@@ -21,7 +21,10 @@ Notation
 Section HoareRules.
   Context {J I: WfRel}.
   Context {Pt Ps : prog rtl_lang}.
-  Context {C : Chain (fsim_lfp J I Pt Ps)}.
+
+  Implicit Type C : Chain (fsim_lfp J I Pt Ps).
+  Context {C}.
+
   Context {ft : rtl_function} {j: J} {i: I} {fs : rtl_function}.
 
   Lemma frame F P Q:
@@ -44,51 +47,5 @@ Section HoareRules.
     iApply ("H" with "[Hpre] [Hpost]").
     - by iApply "HP".
     - iIntros (vt vs) "HQ'". iApply "Hpost". by iApply "HQ".
-  Qed.
-
-  Local Definition hoare_ind_inv Inv
-    (st: pstate rtl_lang) (j': J) (i': I) (ss : pstate rtl_lang)
-    (ϕ: val -> val -> rProp) : rProp :=
-    ∃ ft fs valt vals P Ψ,
-      ⌜st = ([], CallState ft valt) ∧
-       ss = ([], CallState fs vals)⌟ ∗
-      ⌜Inv P ft j' i' fs Ψ⌟ ∗
-      P valt vals ∗
-      (∀ vt vs, Ψ vt vs -∗ ϕ vt vs).
-
-  Lemma hoare_ind Inv P Q:
-    □ (∀ C P ft j i fs Q valt vals Ψ,
-         □ (∀ P ft j' i' fs Q,
-              ⌜j ⊏ j'⌟ -∗
-              ⌜i ⊏ i'⌟ -∗
-              ⌜Inv P ft j i fs Q⌟ -∗
-              [Pt, Ps, C] {{ P }} ft <{j', i'}= fs {{ Q }}
-         ) -∗
-         ⌜Inv P ft j i fs Q⌟ -∗
-         P valt vals -∗
-         (∀ vt vs, Q vt vs -∗ Ψ vt vs) -∗
-         [Pt, Ps, C] ([], CallState ft valt) <{j, i}= ([], CallState fs vals) {{ Ψ }}
-    ) -∗
-    ⌜Inv P ft j i fs Q⌟ -∗
-    [Pt, Ps, C] {{ P }} ft <{j, i}= fs {{ Q }}.
-  Proof using Type.
-    iIntros "#RIH %HInv !>".
-    iIntros (valt vals Ψ) "HPre HPost".
-    iApply (coind (hoare_ind_inv Inv)).
-    - clear.
-      iIntros "!>" (C st j i ss Ψ) "#CIH".
-      iIntros "(%ft & %fs & %valt & %vals & %P & %Q & %H & Hinv & Hpre & Hpost)".
-      destruct H as (-> & ->).
-      iApply ("RIH" with "[] Hinv Hpre Hpost").
-      clear.
-      iIntros "!>" (P ft j' i' fs Q Hj Hi Hinv).
-      iIntros "!>" (valt vals Ψ) "HPre HPost".
-      iApply ("CIH").
-      + by iPureIntro.
-      + by iPureIntro.
-      + iExists ft, fs, valt, vals, P, Q. iFrame. iPureIntro.
-        by split_and!.
-    - iExists ft, fs, valt, vals, P, Q. iFrame. iPureIntro.
-      by split_and!.
   Qed.
 End HoareRules.
