theories/RTL/Rules/SimRules.v
@@ -4,5 +4,5 @@ From RSL.RTL Require Export RTL Semantics.
 
 From RSL.RTL.Rules Require Export Hoare.
 From RSL.RTL.Rules Require Export TargetRules SourceRules.
-From RSL.RTL.Rules Require Export ExploitSourceRules.
+From RSL.RTL.Rules Require Export ExploitSourceRules FailSourceRules.
 From RSL.RTL.Rules Require Export SyncRules.
